Post-condition for ind_cca::encapsulate

libcrux-ml-kem/src/ind_cca.rs
@@ -44,7 +44,7 @@ pub(crate) mod instantiations;
     ${private_key.len()} == Spec.MLKEM.v_CPA_PRIVATE_KEY_SIZE $K /\\
     ${public_key.len()} == Spec.MLKEM.v_CPA_PUBLIC_KEY_SIZE $K /\\
     ${implicit_rejection_value.len()} == Spec.MLKEM.v_SHARED_SECRET_SIZE"))]
-#[hax_lib::ensures(|result| fstar!("result == Seq.append $private_key (
+#[hax_lib::ensures(|result| fstar!("$result == Seq.append $private_key (
                                               Seq.append $public_key (
                                               Seq.append (Spec.Utils.v_H $public_key) 
                                                   $implicit_rejection_value))"))]
@@ -64,24 +64,24 @@ fn serialize_kem_secret_key<const K: usize, const SERIALIZED_KEY_LEN: usize, Has
     out[pointer..pointer + implicit_rejection_value.len()]
         .copy_from_slice(implicit_rejection_value);
     hax_lib::fstar!("let open Spec.Utils in
-        assert (Seq.slice out 0 (v #usize_inttype (Spec.MLKEM.v_CPA_PRIVATE_KEY_SIZE v_K)) `Seq.equal` private_key);
-        assert (Seq.slice out (v #usize_inttype (Spec.MLKEM.v_CPA_PRIVATE_KEY_SIZE v_K))
-                                (v #usize_inttype (Spec.MLKEM.v_CPA_PRIVATE_KEY_SIZE v_K +! Spec.MLKEM.v_CPA_PUBLIC_KEY_SIZE v_K)) `Seq.equal` public_key);
-        assert (Seq.slice out (v #usize_inttype (Spec.MLKEM.v_CPA_PRIVATE_KEY_SIZE v_K +!
-                                                Spec.MLKEM.v_CPA_PUBLIC_KEY_SIZE v_K))
-                                (v #usize_inttype (Spec.MLKEM.v_CPA_PRIVATE_KEY_SIZE v_K +!
-                                                Spec.MLKEM.v_CPA_PUBLIC_KEY_SIZE v_K +!
+        assert (Seq.slice $out 0 (v #usize_inttype (Spec.MLKEM.v_CPA_PRIVATE_KEY_SIZE $K)) `Seq.equal` $private_key);
+        assert (Seq.slice $out (v #usize_inttype (Spec.MLKEM.v_CPA_PRIVATE_KEY_SIZE $K))
+                                (v #usize_inttype (Spec.MLKEM.v_CPA_PRIVATE_KEY_SIZE $K +! Spec.MLKEM.v_CPA_PUBLIC_KEY_SIZE $K)) `Seq.equal` $public_key);
+        assert (Seq.slice $out (v #usize_inttype (Spec.MLKEM.v_CPA_PRIVATE_KEY_SIZE $K +!
+                                                Spec.MLKEM.v_CPA_PUBLIC_KEY_SIZE $K))
+                                (v #usize_inttype (Spec.MLKEM.v_CPA_PRIVATE_KEY_SIZE $K +!
+                                                Spec.MLKEM.v_CPA_PUBLIC_KEY_SIZE $K +!
                                                 Libcrux_ml_kem.Constants.v_H_DIGEST_SIZE))
-                `Seq.equal` Libcrux_ml_kem.Hash_functions.f_H #v_Hasher #v_K public_key);
-        assert (Seq.slice out (v #usize_inttype (Spec.MLKEM.v_CPA_PRIVATE_KEY_SIZE v_K +!
-                                                Spec.MLKEM.v_CPA_PUBLIC_KEY_SIZE v_K +!
+                `Seq.equal` Libcrux_ml_kem.Hash_functions.f_H #v_Hasher #$K $public_key);
+        assert (Seq.slice $out (v #usize_inttype (Spec.MLKEM.v_CPA_PRIVATE_KEY_SIZE $K +!
+                                                Spec.MLKEM.v_CPA_PUBLIC_KEY_SIZE $K +!
                                                 Libcrux_ml_kem.Constants.v_H_DIGEST_SIZE))
-                                (v #usize_inttype (Spec.MLKEM.v_CPA_PRIVATE_KEY_SIZE v_K +!
-                                                Spec.MLKEM.v_CPA_PUBLIC_KEY_SIZE v_K +!
+                                (v #usize_inttype (Spec.MLKEM.v_CPA_PRIVATE_KEY_SIZE $K +!
+                                                Spec.MLKEM.v_CPA_PUBLIC_KEY_SIZE $K +!
                                                 Libcrux_ml_kem.Constants.v_H_DIGEST_SIZE +!
                                                 Spec.MLKEM.v_SHARED_SECRET_SIZE))
-                == implicit_rejection_value);
-        lemma_slice_append_4 out private_key public_key (Libcrux_ml_kem.Hash_functions.f_H #v_Hasher #v_K public_key) implicit_rejection_value");
+                == $implicit_rejection_value);
+        lemma_slice_append_4 $out $private_key $public_key (Libcrux_ml_kem.Hash_functions.f_H #v_Hasher #$K $public_key) $implicit_rejection_value");
     out
 }
 
@@ -175,6 +175,8 @@ fn generate_keypair<
     $ETA1_RANDOMNESS_SIZE == Spec.MLKEM.v_ETA1_RANDOMNESS_SIZE $K /\\
     $ETA2 == Spec.MLKEM.v_ETA2 $K /\\
     $ETA2_RANDOMNESS_SIZE == Spec.MLKEM.v_ETA2_RANDOMNESS_SIZE $K"))]
+#[hax_lib::ensures(|result| fstar!("(${result}._1.f_value, ${result}._2) == 
+    Spec.MLKEM.ind_cca_encapsulate $K ${public_key}.f_value $randomness"))] 
 fn encapsulate<
     const K: usize,
     const CIPHERTEXT_SIZE: usize,
@@ -199,6 +201,9 @@ fn encapsulate<
     let randomness = Scheme::entropy_preprocess::<K, Hasher>(&randomness);
     let mut to_hash: [u8; 2 * H_DIGEST_SIZE] = into_padded_array(&randomness);
     to_hash[H_DIGEST_SIZE..].copy_from_slice(&Hasher::H(public_key.as_slice()));
+    hax_lib::fstar!("assert (Seq.slice $to_hash 0 (v Libcrux_ml_kem.Constants.v_H_DIGEST_SIZE) == $randomness);
+        lemma_slice_append $to_hash $randomness (Libcrux_ml_kem.Hash_functions.f_H #v_Hasher #$K ${public_key}.f_value);
+        assert ($to_hash == concat $randomness (Libcrux_ml_kem.Hash_functions.f_H #v_Hasher #$K ${public_key}.f_value))");
 
     let hashed = Hasher::G(&to_hash);
     let (shared_secret, pseudorandomness) = hashed.split_at(SHARED_SECRET_SIZE);
@@ -532,6 +537,7 @@ pub mod unpacked {
 #[hax_lib::attributes]
 pub(crate) trait Variant {
     #[requires(shared_secret.len() == 32)]
+    #[ensures(|res| fstar!("$res == $shared_secret"))]
     fn kdf<const K: usize, const CIPHERTEXT_SIZE: usize, Hasher: Hash<K>>(
         shared_secret: &[u8],
         ciphertext: &MlKemCiphertext<CIPHERTEXT_SIZE>,
@@ -580,6 +586,8 @@ pub(crate) struct MlKem {}
 impl Variant for MlKem {
     #[inline(always)]
     #[requires(shared_secret.len() == 32)]
+    // Output name has be `out1` https://github.com/hacspec/hax/issues/832
+    #[ensures(|out1| fstar!("$out1 == $shared_secret"))]
     fn kdf<const K: usize, const CIPHERTEXT_SIZE: usize, Hasher: Hash<K>>(
         shared_secret: &[u8],
         _: &MlKemCiphertext<CIPHERTEXT_SIZE>,
