libcrux-ml-kem/proofs/fstar/extraction/Libcrux_ml_kem.Utils.fsti
@@ -7,4 +7,7 @@ open FStar.Mul
 val into_padded_array (v_LEN: usize) (slice: t_Slice u8)
     : Prims.Pure (t_Array u8 v_LEN)
       (requires (Core.Slice.impl__len #u8 slice <: usize) <=. v_LEN)
-      (fun _ -> Prims.l_True)
+      (ensures
+        fun res ->
+          let res:t_Array u8 v_LEN = res in
+          Seq.slice res 0 (Seq.length slice) == slice)
